many modificaction in conc and symbolic interpreter

ver2/interpreter.v
@@ -13,14 +13,14 @@ Definition EVMByteSize: nat := 8.
 Definition EVMByte := word EVMByteSize. 
 
 (* Word *)
-Definition BytesInWord: nat := 32. 
-Definition EVMWordSize: nat := BytesInWord*EVMByteSize. 
+Definition BytesInEVMWord: nat := 32. 
+Definition EVMWordSize: nat := BytesInEVMWord*EVMByteSize. 
 Definition EVMWord:= word EVMWordSize.
 
 (* Address *)
-Definition ByteInAddr : nat := 20. 
-Definition AddrSize : nat := ByteInAddr*ByteInAddr.
-Definition EVMAddr := word AddrSize.
+Definition ByteInEVMAddr : nat := 20. 
+Definition EVMAddrSize : nat := ByteInEVMAddr*EVMByteSize.
+Definition EVMAddr := word EVMAddrSize.
 
 (* Predefined constants *)
 Definition BZero: EVMByte  := natToWord EVMByteSize 0.
@@ -29,6 +29,10 @@ Definition BOne : EVMByte  := natToWord EVMByteSize 1.
 Definition WZero: EVMWord  := natToWord EVMWordSize 0.
 Definition WOne : EVMWord  := natToWord EVMWordSize 1.
 
+Definition AZero: EVMAddr  := natToWord EVMAddrSize 0.
+Definition AOne : EVMAddr  := natToWord EVMAddrSize 1.
+
+(* Maximum size of the stack *)
 Definition StackSize := 1024.
 
 
@@ -38,8 +42,9 @@ Import EVM_Def.
 
 (*
 
-Stack operation instructions require the context and stack as input,
-they compute a value given the input, and they not modify the state.
+Stack operation instructions: they require only the context and the
+stack as input, they compute a value (to be pushed to the stack) given
+the input.
 
 *)
 
@@ -92,11 +97,65 @@ Inductive stack_op_instr :=
 | BASEFEE.
 
 
+Definition eqb_stack_op_instr (a b: stack_op_instr) : bool :=
+  match a,b with
+  | ADD,ADD => true
+  | MUL,MUL => true
+  | SUB,SUB => true
+  | DIV,DIV => true
+  | SDIV,SDIV => true
+  | MOD,MOD => true
+  | SMOD,SMOD => true
+  | ADDMOD,ADDMOD => true
+  | MULMOD,MULMOD => true
+  | EXP,EXP => true
+  | SIGNEXTEND,SIGNEXTEND => true
+  | LT,LT => true
+  | GT,GT => true
+  | SLT,SLT => true
+  | SGT,SGT => true
+  | EQ,EQ => true
+  | ISZERO,ISZERO => true
+  | AND,AND => true
+  | OR,OR => true
+  | XOR,XOR => true
+  | NOT,NOT => true
+  | BYTE,BYTE => true
+  | SHL,SHL => true
+  | SHR,SHR => true
+  | SAR,SAR => true
+  | ADDRESS,ADDRESS => true
+  | BALANCE,BALANCE => true
+  | ORIGIN,ORIGIN => true
+  | CALLER,CALLER => true
+  | CALLVALUE,CALLVALUE => true
+  | CALLDATALOAD,CALLDATALOAD => true
+  | CALLDATASIZE,CALLDATASIZE => true
+  | GASPRICE,GASPRICE => true
+  | EXTCODESIZE,EXTCODESIZE => true
+  | RETURNDATASIZE,RETURNDATASIZE => true
+  | EXTCODEHASH,EXTCODEHASH => true
+  | BLOCKHASH,BLOCKHASH => true
+  | COINBASE,COINBASE => true
+  | TIMESTAMP,TIMESTAMP => true
+  | NUMBER,NUMBER => true
+  | DIFFICULTY,DIFFICULTY => true
+  | GASLIMIT,GASLIMIT => true
+  | CHAINID,CHAINID => true
+  | SELFBALANCE,SELFBALANCE => true
+  | BASEFEE,BASEFEE => true
+  | CODESIZE,CODESIZE => true
+  | _,_ => false
+  end.
+
+Notation "m '=?i' n" := (eqb_stack_op_instr m n) (at level 100).
+
+
 (*
 
-Instructions are (1) the basic stack manipulation ones -- PUSH, POP,
-DUP and SWAP; (2) instruction that operate on memory; and (3) the
-stack operations above.
+Instructions: (1) the basic stack manipulation ones -- PUSH, POP, DUP
+and SWAP; (2) instruction that operate on memory/store; and (3) the
+stack operation instructions above.
 
 *)
 
@@ -116,36 +175,36 @@ Inductive instr :=
 | OpInstr (label: stack_op_instr).
 
 
-(* a block is a list instructions *)
-Definition block := list instr.  
+(* A block is a list instructions *)
+Definition block : Type := list instr.  
 
-(* stack is a list of EVMWord *)
-Definition stack := list EVMWord.
 
-(* 
+(*** Execution State and its auxiliary data-structures ***)
 
-Memory is a mapping from EVMWord to EVMByte. We do not models its 
+(* Stack is a list of EVMWord *)
+Definition stack : Type := list EVMWord.
+Definition empty_stack : stack := [].
 
-*)
-Definition memory := EVMWord -> EVMByte.
+(* Memory is a mapping from EVMWord to EVMByte. We do not keep its
+accessed size, i.e., don't handle memory expansion, because we don't
+track gas consumption. *)
+Definition memory : Type := EVMWord -> EVMByte.
+Definition empty_memory : memory := fun _ => BZero.
 
-(* store is a function from addresses to values *)
-Definition storage := EVMWord -> EVMWord.
+(* Storage is a function from EVMWord (key) to values EVMWord
+(value). We don't model the warm/cold properies since we don't track
+gas consumption *)
+Definition storage : Type := EVMWord -> EVMWord.
+Definition empty_storage : storage := fun _ => WZero.
 
 (*
 
-Context encapsulates all contract/blockchain information, it never
-changes durin the execution of a block.
-
-We can extend it use to model operations that are not implemented, as
-far as these operations are not use in a rule optimization. This can
-be done simply by specifying the function in the context, and the
-implementation simply forwards to that function. For example, below we
-do this for KECCAK256 whose implementation is not really needed.
+Context is a strute that we use to encapsulates all
+contract/blockchain information, and operations that we don't want to
+implement such as KECCAK256 (correctness will be shown for any value
+of such operations). The structure is immutable.
 
 *)
-
-(* the use of _ctx_ is just to avoid conflicts with other data types *)
 
 Inductive code_info :=
 | CodeInfo (size : nat) (content : word size) (hash : EVMWord).
@@ -174,240 +233,197 @@ Ctx
   (chainid : EVMWord)
   (basefee : EVMWord)
   (keccak256 : memory -> EVMWord -> EVMWord -> EVMWord)
-  (_extra_1 : unit)
-  (_extra_2 : unit)
-  (_extra_3 : unit)
-  (_extra_4 : unit)
-  (_extra_5 : unit).
+  (_extra_1 : nat)
+  (_extra_2 : nat)
+  (_extra_3 : nat)
+  (_extra_4 : nat)
+  (_extra_5 : nat).
 
+
+Definition empty_context : context :=
+ Ctx
+  AZero (* (address : EVMAddr) *)
+  (fun _ => WZero) (* (balance : EVMAddr -> EVMWord) *)
+  AZero (* (origin : EVMAddr) *)
+  AZero (* (caller : EVMAddr) *)
+  WZero (* (callvalue : EVMWord) *)
+  (Chunk 0 WO) (* (data: chunk) *)
+  (fun _ => CodeInfo 0 WO WZero) (* (code : EVMAddr -> code_info )  *)
+  WZero (* (gasprice : EVMWord) *)
+  (Chunk 0 WO) (* (outdata: chunk) *)
+  (fun _ => BlockInfo 0 WO WZero WZero) (* (blokcs : EVMWord -> block_info) *)
+  AZero (* (miner : EVMAddr) *)
+  WZero (* (currblock : EVMWord) *)
+  WZero (* (gaslimit : EVMWord) *)
+  WZero (* (chainid : EVMWord) *)
+  WZero (* (basefee : EVMWord) *)
+  (fun _ _ _ => WZero) (* (keccak256 : memory -> EVMWord -> EVMWord -> EVMWord) *)
+  0 (* (_extra_1 : nat) *)
+  0 (* (_extra_2 : nat) *)
+  0 (* (_extra_3 : nat) *)
+  0 (* (_extra_4 : nat) *)
+  0. (* (_extra_5 : nat) *)
+    
 (* Ctx _ _ _ _ _ _ _ _ _ _ _ _ _ _ _ _ _ *)
 
-Definition get_address (c : context) :=
+Definition get_address_ctx (c : context) :=
   match c with
   | Ctx x _ _ _ _ _ _ _ _ _ _ _ _ _ _ _ _ _ _ _ _ => x
   end.
 
-Definition get_balance (c : context) :=
+Definition get_balance_ctx (c : context) :=
   match c with
   | Ctx _ x _ _ _ _ _ _ _ _ _ _ _ _ _ _ _ _ _ _ _ => x
   end.
 
-Definition get_origin (c : context) :=
+Definition get_origin_ctx (c : context) :=
   match c with
   | Ctx _ _ x _ _ _ _ _ _ _ _ _ _ _ _ _ _ _ _ _ _ => x
   end.
 
-Definition get_caller (c : context) :=
+Definition get_caller_ctx (c : context) :=
   match c with
   | Ctx _ _ _ x _ _ _ _ _ _ _ _ _ _ _ _ _ _ _ _ _ => x
   end.
 
-Definition get_callvalue (c : context) :=
+Definition get_callvalue_ctx (c : context) :=
   match c with
   | Ctx _ _ _ _ x _ _ _ _ _ _ _ _ _ _ _ _ _ _ _ _ => x
   end.
 
-Definition get_data (c : context) :=
+Definition get_data_ctx (c : context) :=
   match c with
   | Ctx _ _ _ _ _ x _ _ _ _ _ _ _ _ _ _ _ _ _ _ _ => x
   end.
 
-Definition get_code (c : context) :=
+Definition get_code_ctx (c : context) :=
   match c with
   | Ctx _ _ _ _ _ _ x _ _ _ _ _ _ _ _ _ _ _ _ _ _ => x
   end.
 
-Definition get_gasprice (c : context) :=
+Definition get_gasprice_ctx (c : context) :=
   match c with
   | Ctx _ _ _ _ _ _ _ x _ _ _ _ _ _ _ _ _ _ _ _ _ => x
   end.
 
-Definition get_outdata (c : context) :=
+Definition get_outdata_ctx (c : context) :=
   match c with
   | Ctx _ _ _ _ _ _ _ _ x _ _ _ _ _ _ _ _ _ _ _ _ => x
   end.
 
-Definition get_blokcs (c : context) :=
+Definition get_blokcs_ctx (c : context) :=
   match c with
   | Ctx _ _ _ _ _ _ _ _ _ x _ _ _ _ _ _ _ _ _ _ _ => x
   end.
 
-Definition get_miner (c : context) :=
+Definition get_miner_ctx (c : context) :=
   match c with
   | Ctx _ _ _ _ _ _ _ _ _ _ x _ _ _ _ _ _ _ _ _ _ => x
   end.
 
-Definition get_currblock (c : context) :=
+Definition get_currblock_ctx (c : context) :=
   match c with
   | Ctx _ _ _ _ _ _ _ _ _ _ _ x _ _ _ _ _ _ _ _ _ => x
   end.
 
-Definition get_gaslimit (c : context) :=
+Definition get_gaslimit_ctx (c : context) :=
   match c with
   | Ctx _ _ _ _ _ _ _ _ _ _ _ _ x _ _ _ _ _ _ _ _ => x
   end.
 
-Definition get_chainid (c : context) :=
+Definition get_chainid_ctx (c : context) :=
   match c with
   | Ctx _ _ _ _ _ _ _ _ _ _ _ _ _ x _ _ _ _ _ _ _ => x
   end.
 
-Definition get_basefee (c : context) :=
+Definition get_basefee_ctx (c : context) :=
   match c with
   | Ctx _ _ _ _ _ _ _ _ _ _ _ _ _ _ x _ _ _ _ _ _ => x
   end.
 
-Definition get_keccak256 (c : context) :=
+Definition get_keccak256_ctx (c : context) :=
   match c with
   | Ctx _ _ _ _ _ _ _ _ _ _ _ _ _ _ _ x _ _ _ _ _ => x
   end.
 
 
-Definition comm_op (f : context -> list EVMWord -> EVMWord)  : Prop :=
-  forall (a b : EVMWord) (ctx : context),
-    f ctx [a;b] = f ctx [b;a].
-
-
-Definition coherent_stack_op (n : nat) (f: context -> list EVMWord -> option EVMWord) : Prop :=
-forall  (ctx : context) (l: list EVMWord), length l = n -> exists (v: EVMWord), f ctx l = Some v.
-
-Inductive op_impl :=
-| OpImp (n : nat) (f : context -> list EVMWord -> EVMWord) (H : option (comm_op f)).
-
-
-Definition eq_stack_op_instr (a b: stack_op_instr) : bool :=
-    match a, b with
-    | ADD,ADD => true
-    | MUL,MUL => true
-    | SUB,SUB => true
-    | DIV,DIV => true
-    | SDIV,SDIV => true
-    | MOD,MOD => true
-    | SMOD,SMOD => true
-    | ADDMOD,ADDMOD => true
-    | MULMOD,MULMOD => true
-    | EXP,EXP => true
-    | SIGNEXTEND,SIGNEXTEND => true
-    | LT,LT => true
-    | GT,GT => true
-    | SLT,SLT => true
-    | SGT,SGT => true
-    | EQ,EQ => true
-    | ISZERO,ISZERO => true
-    | AND,AND => true
-    | OR,OR => true
-    | XOR,XOR => true
-    | NOT,NOT => true
-    | BYTE,BYTE => true
-    | SHL,SHL => true
-    | SHR,SHR => true
-    | SAR,SAR => true
-    | ADDRESS,ADDRESS => true
-    | BALANCE,BALANCE => true
-    | ORIGIN,ORIGIN => true
-    | CALLER,CALLER => true
-    | CALLVALUE,CALLVALUE => true
-    | CALLDATALOAD,CALLDATALOAD => true
-    | CALLDATASIZE,CALLDATASIZE => true
-    | GASPRICE,GASPRICE => true
-    | EXTCODESIZE,EXTCODESIZE => true
-    | RETURNDATASIZE,RETURNDATASIZE => true
-    | EXTCODEHASH,EXTCODEHASH => true
-    | BLOCKHASH,BLOCKHASH => true
-    | COINBASE,COINBASE => true
-    | TIMESTAMP,TIMESTAMP => true
-    | NUMBER,NUMBER => true
-    | DIFFICULTY,DIFFICULTY => true
-    | GASLIMIT,GASLIMIT => true
-    | CHAINID,CHAINID => true
-    | SELFBALANCE,SELFBALANCE => true
-    | BASEFEE,BASEFEE => true
-    | CODESIZE,CODESIZE => true
-    | _,_ => false
-    end.
-
-Notation "m '=?i' n" := (eq_stack_op_instr m n) (at level 100).
-
-
-(****** Concrete state ******)
 
 Inductive state :=
- | ExState (stk: stack) (mem: memory) (stg: storage) (ctx :context).
+| ExState (stk: stack) (mem: memory) (stg: storage) (ctx :context).
+
+Definition empty_state := ExState empty_stack empty_memory empty_storage.
 
 
 Definition get_stack_st (st: state) : stack :=
-match st with
-| ExState stk _ _  => stk
-end.
+  match st with
+  | ExState stk _ _ _ => stk
+  end.
 
-Definition set_stack_st (st: state) (stk: stack) 
-  : state :=
-match st with
-| ExState _ mem strg ctx => ExState stk mem strg ctx
-end.
+Definition set_stack_st (st: state) (stk: stack) : state :=
+  match st with
+  | ExState _ mem strg ctx => ExState stk mem strg ctx
+  end.
 
 Definition get_memory_st (st: state) : memory :=
-match st with
-| ExState _ mem _ _=> mem
-end.
+  match st with
+  | ExState _ mem _ _=> mem
+  end.
 
-Definition set_memory_st (st: state) (mem: memory) 
-  : state :=
-match st with
-| ExState stk _ strg ctx => ExState stk mem strg ctx
-end.
+Definition set_memory_st (st: state) (mem: memory) : state :=
+  match st with
+  | ExState stk _ strg ctx => ExState stk mem strg ctx
+  end.
 
 Definition get_store_st (st: state) : storage :=
-match st with
-| ExState _ _ strg _ => strg
-end.
+  match st with
+  | ExState _ _ strg _ => strg
+  end.
 
-Definition set_store_st (st: state) (strg: storage)
-  : state :=
-match st with
-| ExState stk mem _ ctx => ExState stk mem strg ctx
-end.
+Definition set_store_st (st: state) (strg: storage) : state :=
+  match st with
+  | ExState stk mem _ ctx => ExState stk mem strg ctx
+  end.
 
 Definition get_context_st (st: state) : context :=
-match st with
-| ExState _ _ _ ctx => ctx
-end.
+  match st with
+  | ExState _ _ _ ctx => ctx
+  end.
 
-Definition set_context_st (st: state) (ctx: context)
-  : state :=
-match st with
-| ExState stk mem strg _ => ExState stk mem strg ctx
-end.
-
+Definition set_context_st (st: state) (ctx: context) : state :=
+  match st with
+  | ExState stk mem strg _ => ExState stk mem strg ctx
+  end.
+  
 (************)
 
-(* ================================================================= *)
-(** ** Definition of maps *)
+
+
+(* Some stack operation instructions are commutative, a property that
+might be used when optimizing a block. The following definition models
+this property. *)
+Definition commutative_op (f : context -> list EVMWord -> EVMWord) : Prop :=
+  forall (a b : EVMWord) (ctx : context), f ctx [a;b] = f ctx [b;a].
+
+(* An implementation of a stack operation instructions *)
+Inductive stack_op_impl :=
+| OpImp (n : nat) (f : context -> list EVMWord -> EVMWord) (H : option (commutative_op f)).
+
 
 (* The maps here link an opcode (oper_label) to an operator *)
-
  
 Definition map (K V : Type) : Type := K -> option V.
 
-Definition empty_imap {A : Type} : map stack_op_instr A := (fun _ => None).
-Definition updatei {A : Type} (m : map stack_op_instr A) 
-    (x : stack_op_instr) (v : A) :=
-fun x' => if x =?i x' then Some v else m x'.
+Definition stack_op_instr_map := map stack_op_instr stack_op_impl.
 
-Notation "x '|->i' v ';' m" := (updatei m x v)
-  (at level 100, v at next level, right associativity).
-Notation "x '|->i' v" := (updatei empty_imap x v)
-  (at level 100).
-  
-Definition empty_nmap {A : Type} : map nat A := (fun _ => None).
-Definition updaten {A : Type} (m : map nat A) (x : nat) (v : A) :=
-  fun x' => if x =? x' then Some v else m x'.
-Notation "x '|->n' v ';' m" := (updaten m x v)
-  (at level 100, v at next level, right associativity).
-Notation "x '|->n' v" := (updaten empty_nmap x v)
-  (at level 100).
-    
-Definition stack_op_map := map stack_op_instr op_impl.
+Definition empty_imap {A : Type} : map stack_op_instr A :=
+  (fun _ =>  None).
+
+Definition updatei {A : Type} (m : map stack_op_instr A) (x : stack_op_instr) (v : A) :=
+  fun x' => if x =?i x' then Some v else m x'.
+
+Notation "x '|->i' v ';' m" := (updatei m x v) (at level 100, v at next level, right associativity).
+Notation "x '|->i' v" := (updatei empty_imap x v) (at level 100).
+
 
 
 (******* stack manipulation operators ********)
@@ -421,59 +437,53 @@ Definition skipn_e {A: Type} (n:nat) (l:list A) : option (list A) :=
 
 (* Polymorphic versions for manipulating the stack *)
 Definition push {T : Type} (v : T) (stk : list T) : option (list T) :=
-if List.length(stk) <? StackSize then Some (v :: stk) else None.
+  if List.length(stk) <? StackSize then Some (v :: stk) else None.
 
 Definition pop {T : Type} (stk: list T): option (list T) :=
-match stk with
- | x::stk' => Some stk'
- | _ => None
-end.
-
-Definition dup {T: Type} (k : nat) (stk: list T) : option (list T) :=
-if ((k =? 0) || (16 <? k) || (StackSize <=? List.length(stk))) then None
-else match nth_error stk (pred k) with
-  | None => None
-  | Some x => Some (x::stk)
+  match stk with
+  | x::stk' => Some stk'
+  | _ => None
   end.
 
+Definition dup {T: Type} (k : nat) (stk: list T) : option (list T) :=
+  if ((k =? 0) || (16 <? k) || (StackSize <=? List.length(stk))) then None
+  else match nth_error stk (pred k) with
+       | None => None
+       | Some x => Some (x::stk)
+       end.
+
 Definition swap {T: Type} (k : nat) (stk: list T) : option (list T) :=
-if ((k =? 0) || (16 <? k)) then None
-else match (nth_error stk k, stk) with
-     | (Some v, h::t) => Some ([v] ++ ((firstn (k-1) t)) 
-                               ++ [h] ++ (skipn (k+1) stk))
-     | _  => None
-     end.
+  if ((k =? 0) || (16 <? k)) then None
+  else match (nth_error stk k, stk) with
+       | (Some v, h::t) => Some ([v] ++ ((firstn (k-1) t)) ++ [h] ++ (skipn (k+1) stk))
+       | _ => None
+       end.
 
 (* version operating on execution states *)
-Definition push_c (v : EVMWord) (st : state)
-  : option state :=
-let stk := get_stack_st st in
-match push v stk with
-| None => None
-| Some stk' => Some (set_stack_st st stk')
-end.
+Definition push_c (v : EVMWord) (st : state) : option state :=
+  let stk := get_stack_st st in
+  match push v stk with
+  | None => None
+  | Some stk' => Some (set_stack_st st stk')
+  end.
 
-Definition pop_c (st : state): option state :=
-let stk := get_stack_st st in
-match pop stk with
- | None => None
- | Some stk' => Some (set_stack_st st stk')
-end.
+Definition pop_c (st : state): option state := let stk := get_stack_st
+st in match pop stk with | None => None | Some stk' => Some
+(set_stack_st st stk') end.
 
-Definition dup_c (k : nat) (st : state) : option state  :=
-let stk := get_stack_st st in
-match dup k stk with
- | None => None
- | Some stk' => Some (set_stack_st st stk')
-end.
+Definition dup_c (k : nat) (st : state) : option state :=
+  let stk := get_stack_st st in
+  match dup k stk with
+  | None => None
+  | Some stk' => Some (set_stack_st st stk')
+  end.
 
 Definition swap_c (k : nat) (st : state) : option state :=
-let stk := get_stack_st st in
-match swap k stk with
- | None => None
- | Some stk' => Some (set_stack_st st stk')
-end.
-
+  let stk := get_stack_st st in
+  match swap k stk with
+  | None => None
+  | Some stk' => Some (set_stack_st st stk')
+  end.
 
 Definition mload_ (mem : memory) (offset : EVMWord) :=
   fix mload_fix (n : nat) : word (n * 8) :=
@@ -485,34 +495,31 @@ Definition mload_ (mem : memory) (offset : EVMWord) :=
 Definition mload (mem : memory) (offset : EVMWord) : EVMWord :=
   mload_ mem offset 32.
   
-Definition mstore8 (mem : memory) (offset : EVMWord) (value : EVMByte) :=
-  fun offset' => if (weqb offset' offset) then value else mem offset'.
+Definition mstore8 (mem : memory) (offset : EVMWord) (value : EVMByte)
+  := fun offset' => if (weqb offset' offset) then value else mem
+  offset'.
 
 Fixpoint mstore {sz : nat} (mem : memory) : (word sz) -> EVMWord -> (EVMWord -> EVMByte) :=
   match sz with
   | S (S (S (S (S (S (S (S sz1'))))))) =>
       fun value offset =>
-         let byte := split1 8 sz1' value in
-         let mem' := fun offset' => if (weqb offset' offset) then byte else mem offset' in
-         mstore mem (bbv.Word.split2 8 sz1' value) (wplus offset WOne)
+        let byte := split1 8 sz1' value in
+        let mem' := fun offset' => if (weqb offset' offset) then byte else mem offset' in
+        mstore mem (bbv.Word.split2 8 sz1' value) (wplus offset WOne)
   | _ => fun _ _ => mem
   end.
 
-
-Definition sload (strg : storage) (key : EVMWord) :=
-  strg key.
+Definition sload (strg : storage) (key : EVMWord) := strg key.
 
 Definition sstore (strg : storage) (key : EVMWord) (value : EVMWord) :=
   fun key' => if (weqb key' key) then value else strg key'.
 
 Definition mload_c (st : state) : option state :=
   match get_stack_st st with
-  | offset::stk =>
-      let v := mload (get_memory_st st) offset in
-      let st' := set_stack_st st (v::stk) in 
-      Some st'
-  | _ => None
-  end.
+  | offset::stk => let v := mload (get_memory_st st) offset in
+                   let st' := set_stack_st st (v::stk) in
+                   Some st'
+  | _ => None end.
 
 Definition mstore8_c (st : state) : option state :=
   match get_stack_st st with
@@ -521,27 +528,23 @@ Definition mstore8_c (st : state) : option state :=
       let st' := set_memory_st st mem in
       let st'' := set_stack_st st' stk in
       Some st''
-  | _ => None
-  end.
+  | _ => None end.
 
 Definition mstore_c (st : state) : option state :=
   match get_stack_st st with
   | offset::value::stk =>
       let mem := mstore (get_memory_st st) offset value in
       let st' := set_memory_st st mem in
-      let st'' := set_stack_st st' stk in
-      Some st''
-  | _ => None
-  end.
+      let st'' := set_stack_st st' stk in Some st''
+  | _ => None end.
 
 Definition sload_c (st : state) : option state :=
   match get_stack_st st with
   | key::stk =>
       let v := sload (get_store_st st) key in
-      let st' := set_stack_st st (v::stk) in 
+      let st' := set_stack_st st (v::stk) in
       Some st'
-  | _ => None
-  end.
+  | _ => None end.
 
 Definition sstore_c (st : state) : option state :=
   match get_stack_st st with
@@ -550,81 +553,80 @@ Definition sstore_c (st : state) : option state :=
       let st' := set_store_st st strg in
       let st'' := set_stack_st st' stk in
       Some st''
-  | _ => None
-  end.
+  | _ => None end.
 
 (* just return 0 for now *)
 Definition sha3_c (st : state) : option state :=
   match get_stack_st st with
   | offset::size::stk =>
-      let f := get_keccak256 (get_context_st st) in
+      let f := get_keccak256_ctx (get_context_st st) in
       let v := f (get_memory_st st) offset size in
-      let st' := set_stack_st st (v::stk) in 
+      let st' := set_stack_st st (v::stk) in
       Some st'
-  | _ => None
-  end.
+  | _ =>
+None end.
 
-Definition exec_op_c (st : state) (ops : stack_op_map) (label : stack_op_instr) : option state :=
+Definition exec_stack_op_intsr_c (st : state) (ops : stack_op_instr_map) (label : stack_op_instr) : option state :=
   match (ops label) with
   | None => None
-  | Some (OpImp nb_args func _) => 
+  | Some (OpImp nb_args func _) =>
       let stk := get_stack_st st in
       match firstn_e nb_args stk with
       | None => None
-      | Some args => match skipn_e nb_args stk with 
+      | Some args => match skipn_e nb_args stk with
                      | None => None
                      | Some stk' =>
                          let v := func (get_context_st st) args in
-                         Some (set_stack_st st (v :: stk'))
+                         let st':= set_stack_st st (v :: stk') in
+                         Some st'
                      end
       end
   end.
-
+                             
 
 (* Concrete interpreter *)
-Definition evm_exec_instr (inst : instr) (st: state) (ops : stack_op_map) : option state :=
+Definition evm_exec_instr (inst : instr) (st: state) (ops : stack_op_instr_map) : option state :=
   match inst with
   | PUSH size v => push_c (NToWord EVMWordSize v) st
   | POP => pop_c st
   | DUP k => dup_c k st
   | SWAP k => swap_c k st
-  | MLOAD => mload_c st                 
-  | MSTORE8 => mstore8_c st                 
-  | MSTORE => mstore_c st                 
-  | SLOAD => sload_c st                 
+  | MLOAD => mload_c st
+  | MSTORE8 => mstore8_c st
+  | MSTORE => mstore_c st
+  | SLOAD => sload_c st
   | SSTORE => sstore_c st
   | SHA3 => sha3_c st
   | KECCAK256 => sha3_c st
-  | OpInstr label => exec_op_c st ops label
+  | OpInstr label => exec_stack_op_intsr_c st ops label
   end.
 
                
-Fixpoint evm_exec_block (p : block) (st : state)
-  (ops : stack_op_map) : option state :=
+Fixpoint evm_exec_block (p : block) (st : state) (ops : stack_op_instr_map) : option state :=
   match p with
   | [] => Some st
-  | inst::insts' =>
-    match (evm_exec_instr inst st ops) with
-    | None => None
-    | Some st' => evm_exec_block insts' st' ops
-    end
+  | instr::instrs' =>
+      match evm_exec_instr instr st ops with
+      | None => None
+      | Some st' => evm_exec_block instrs' st' ops
+      end
   end.
 
 
 
 
-(* ================================================================= *)
-(** ** Implementation of current instructions *)
+(* =================================================================
+*) (** ** Implementation of current instructions *)
 
 Definition evm_add (ctx : context) (args : list EVMWord) : EVMWord :=
   match args with
-  | [a;b] => (wplus a b)
+  | [a;b] => wplus a b
   | _ => WZero
   end.
 
-Lemma add_comm: comm_op evm_add.
+Lemma add_comm: commutative_op evm_add.
 Proof.
-  unfold comm_op.
+  unfold commutative_op.
   intros.
   unfold evm_add.
   rewrite -> wplus_comm.
@@ -633,20 +635,20 @@ Qed.
         
 Definition evm_mul (ctx : context) (args : list EVMWord) : EVMWord :=
   match args with
-  | [a;b] => (wmult a b)
+  | [a;b] => wmult a b
   | _ => WZero
   end.
 
 
 Definition evm_sub (ctx : context) (args : list EVMWord) : EVMWord :=
   match args with
-  | [a;b] => (wminus a b)
+  | [a;b] => wminus a b
   | _ => WZero
   end.
 
 Definition evm_div (ctx : context) (args : list EVMWord) : EVMWord :=
   match args with
-  | [a;b] => (wdiv a b)
+  | [a;b] => wdiv a b
   | _ => WZero
   end.
 
@@ -667,7 +669,7 @@ Definition evm_mulmod (ctx : context) (args : list EVMWord) : EVMWord :=
 
 Definition evm_exp (ctx : context) (args : list EVMWord) : EVMWord :=
   match args with
-  | [a;b] => (NToWord EVMWordSize (N.pow (wordToN a) (wordToN b)))
+  | [a;b] => NToWord EVMWordSize (N.pow (wordToN a) (wordToN b))
   | _ => WZero
   end.
   
@@ -677,10 +679,9 @@ Definition evm_signextend (ctx : context) (args : list EVMWord) : EVMWord :=
 
 Definition evm_lt (ctx : context) (args : list EVMWord) : EVMWord :=
   match args with
-  | [a;b] => (if (N.ltb (wordToN a) (wordToN b)) then WOne else WZero)
+  | [a;b] => if (N.ltb (wordToN a) (wordToN b)) then WOne else WZero
   | _ => WZero
   end.
-  
 
 Definition evm_gt (ctx : context) (args : list EVMWord) : EVMWord :=
   match args with
@@ -696,7 +697,7 @@ Definition evm_sgt (ctx : context) (args : list EVMWord) : EVMWord :=
 
 Definition evm_eq (ctx : context) (args : list EVMWord) : EVMWord :=
   match args with
-  | [a;b] => (if weqb a b then WOne else WZero)
+  | [a;b] => if weqb a b then WOne else WZero
   | _ => WZero
   end.
   
@@ -708,26 +709,25 @@ Definition evm_iszero (ctx : context) (args : list EVMWord) : EVMWord :=
 
 Definition evm_and (ctx : context) (args : list EVMWord) : EVMWord :=
   match args with
-  | [a;b] => (wand a b)
+  | [a;b] => wand a b
   | _ => WZero
   end.
-  
 
 Definition evm_or (ctx : context) (args : list EVMWord) : EVMWord :=
   match args with
-  | [a;b] => (wor a b)
+  | [a;b] => wor a b
   | _ => WZero
   end.
 
 Definition evm_xor (ctx : context) (args : list EVMWord) : EVMWord :=
   match args with
-  | [a;b] => (wxor a b)
+  | [a;b] => wxor a b
   | _ => WZero
   end.
 
 Definition evm_not (ctx : context) (args : list EVMWord) : EVMWord :=
   match args with
-  | [a] => (wnot a)
+  | [a] => wnot a
   | _ => WZero
   end.
 
@@ -736,13 +736,13 @@ Definition evm_byte (ctx : context) (args : list EVMWord) : EVMWord :=
 
 Definition evm_shl (ctx : context) (args : list EVMWord) : EVMWord :=
   match args with
-  | [a;b] => (wlshift' b (wordToNat a))
+  | [a;b] => wlshift' b (wordToNat a)
   | _ => WZero
   end.
 
 Definition evm_shr (ctx : context) (args : list EVMWord) : EVMWord :=
   match args with
-  | [a;b] => (wrshift' b (wordToNat a))
+  | [a;b] => wrshift' b (wordToNat a)
   | _ => WZero
   end.
 
@@ -801,7 +801,7 @@ Definition evm_difficulty (ctx : context) (args : list EVMWord) : EVMWord :=
   WZero.
 
 Definition evm_gaslimit (ctx : context) (args : list EVMWord) : EVMWord :=
-   WZero.
+  WZero.
 
 Definition evm_chainid (ctx : context) (args : list EVMWord) : EVMWord :=
   WZero.
@@ -813,7 +813,7 @@ Definition evm_basefee (ctx : context) (args : list EVMWord) : EVMWord :=
   WZero.
 
 
-Definition evm_stack_opm : stack_op_map :=
+Definition evm_stack_opm : stack_op_instr_map :=
   ADD |->i OpImp 2 evm_add (Some add_comm);
   MUL |->i OpImp 2 evm_mul None;
   SUB |->i OpImp 2 evm_sub None;
@@ -822,43 +822,43 @@ Definition evm_stack_opm : stack_op_map :=
   MOD |->i OpImp 2 evm_mod None;
   SMOD |->i OpImp 2 evm_smod None;
   ADDMOD |->i OpImp 3 evm_addmod None;
-  MULMOD |->i OpImp 3 evm_mulmod None;
+  MULMOD |->i  OpImp 3 evm_mulmod None;
   EXP |->i OpImp 2 evm_exp None;
-  SIGNEXTEND |->i OpImp 2 evm_signextend None;
+  SIGNEXTEND  |->i OpImp 2 evm_signextend None;
   LT |->i OpImp 2 evm_lt None;
-  GT |->i OpImp 2 evm_gt None;
+  GT  |->i OpImp 2 evm_gt None;
   SLT |->i OpImp 2 evm_slt None;
-  SGT |->i OpImp 2 evm_sgt None;
+  SGT |->i  OpImp 2 evm_sgt None;
   EQ |->i OpImp 2 evm_eq None;
-  ISZERO |->i OpImp 1 evm_iszero None;
+  ISZERO |->i OpImp  1 evm_iszero None;
   AND |->i OpImp 2 evm_and None;
-  OR |->i OpImp 2 evm_or None;
+  OR |->i OpImp 2  evm_or None;
   XOR |->i OpImp 2 evm_xor None;
-  NOT |->i OpImp 1 evm_not None;
+  NOT |->i OpImp 1 evm_not  None;
   BYTE |->i OpImp 2 evm_byte None;
-  SHL |->i OpImp 2 evm_shl None;
+  SHL |->i OpImp 2 evm_shl  None;
   SHR |->i OpImp 2 evm_shr None;
   SAR |->i OpImp 2 evm_sar None;
   ADDRESS |->i OpImp 0 evm_address None;
-  BALANCE |->i OpImp 1 evm_balance None;
+  BALANCE |->i OpImp 1  evm_balance None;
   ORIGIN |->i OpImp 0 evm_origin None;
-  CALLER |->i OpImp 0 evm_caller None;
+  CALLER |->i  OpImp 0 evm_caller None;
   CALLVALUE |->i OpImp 0 evm_callvalue None;
   CALLDATALOAD |->i OpImp 1 evm_calldataload None;
-  CALLDATASIZE |->i OpImp 0 evm_calldatasize None;
-  CODESIZE |->i OpImp 0 evm_codesize None;
+  CALLDATASIZE |->i  OpImp 0 evm_calldatasize None;
+  CODESIZE |->i OpImp 0 evm_codesize  None;
   GASPRICE |->i OpImp 0 evm_gasprice None;
-  EXTCODESIZE |->i OpImp 1 evm_extcodesize None;
-  RETURNDATASIZE |->i OpImp 0 evm_returndatasize None;
-  EXTCODEHASH |->i OpImp 1 evm_extcodehash None;
+  EXTCODESIZE |->i  OpImp 1 evm_extcodesize None;
+  RETURNDATASIZE |->i OpImp 0  evm_returndatasize None;
+  EXTCODEHASH |->i OpImp 1 evm_extcodehash  None;
   BLOCKHASH |->i OpImp 1 evm_blockhash None;
-  COINBASE |->i OpImp 0 evm_coinbase None;
+  COINBASE |->i OpImp  0 evm_coinbase None;
   TIMESTAMP |->i OpImp 0 evm_timestamp None;
   NUMBER |->i OpImp 0 evm_number None;
-  DIFFICULTY |->i OpImp 0 evm_difficulty None;
+  DIFFICULTY |->i OpImp 0  evm_difficulty None;
   GASLIMIT |->i OpImp 0 evm_gaslimit None;
   CHAINID |->i OpImp 0 evm_chainid None;
-  SELFBALANCE |->i OpImp 0 evm_selfbalance None;
+  SELFBALANCE |->i OpImp 0  evm_selfbalance None;
   BASEFEE |->i OpImp 0 evm_basefee None.
  
 
@@ -869,100 +869,114 @@ Inductive sstack_val : Type :=
 | InStackVar (var: nat)
 | FreshVar (var: nat).
 
-Definition sstack := list sstack_val.
-
+Definition sstack : Type := list sstack_val.
+Definition empty_sstack : sstack := [].
 
 (* Symbolic memory *)
 
 Inductive smemory_val : Type :=
-| SymMSTORE  (offset: sstack_val) (value: sstack_val)
+| SymMSTORE (offset: sstack_val) (value: sstack_val)
 | SymMSTORE8 (offset: sstack_val) (value: sstack_val).
-Definition smemory := list smemory_val.
 
-(* Symbolic memory *)
+Definition smemory : Type := list smemory_val.
+Definition empty_smemory : smemory := [].
+
+(* Symbolic storage *)
 
 Inductive sstorage_val : Type :=
 | SymSSTORE (key: sstack_val) (value: sstack_val).
 
-Definition sstorage := list sstorage_val.
+Definition sstorage : Type := list sstorage_val.
+Definition empty_sstorage : sstorage := [].
 
-Definition scontext := unit. (* ctx is not used actually *)
+Inductive scontext :=
+  | SymCtx. 
+Definition empty_scontext : scontext := SymCtx.
 
 Inductive smap_value : Type :=
 | SymBasicVal (val: sstack_val)
 | SymOp (opcode : stack_op_instr) (args : list sstack_val)
 | SymMLOAD (offset: sstack_val) (smem : smemory)
 | SymSLOAD (key: sstack_val) (sstrg : sstorage)
-| SymSHA3  (offset: sstack_val) (size: sstack_val) (sstrg : smemory).
+| SymSHA3 (offset: sstack_val) (size: sstack_val) (sstrg : smemory).
 
-Inductive smap :=
-  SymMap (maxid : nat) (map: list (nat*smap_value)).
+Inductive smap := SymMap (maxid : nat) (map: list (nat*smap_value)).
+Definition empty_smap : smap := SymMap 0 [].
 
 Inductive sstate :=
- | SymExState (instk_height: nat) (sstk: sstack) (smem: smemory) (sstg: sstorage) (sctx : scontext) (sm: smap). 
+| SymExState (instk_height: nat) (sstk: sstack) (smem: smemory) (sstg: sstorage) (sctx : scontext) (sm: smap).
+
+Definition gen_empty_sstate (instk_height: nat) : sstate :=
+  let ids := seq 0 instk_height in
+  let sstk := List.map InStackVar ids in
+  SymExState instk_height sstk empty_smemory empty_sstorage empty_scontext empty_smap.
 
 Definition get_instk_height_sst (sst: sstate) : nat :=
-match sst with
-| SymExState instk_height _ _ _ _ _ => instk_height
-end.
+  match sst with
+  | SymExState instk_height _ _ _ _ _ => instk_height
+  end.
 
 Definition set_instk_height_sst (sst: sstate) (instk_height : nat) : sstate :=
-match sst with
-| SymExState _ sstk smem sstrg sctx sm => SymExState instk_height sstk smem sstrg sctx sm
-end.
+  match sst with
+  | SymExState _ sstk smem sstrg sctx sm => SymExState instk_height sstk smem sstrg sctx sm
+  end.
 
 Definition get_sstack_sst (sst: sstate) : sstack :=
-match sst with
-| SymExState _ sstk _ _ _ _ => sstk
-end.
+  match sst with
+  | SymExState _ sstk _ _ _ _ => sstk
+  end.
 
 Definition set_sstack_sst (sst: sstate) (sstk: sstack) : sstate :=
-match sst with
-| SymExState instk_height _ smem sstrg sctx sm => SymExState instk_height sstk smem sstrg sctx sm
-end.
+  match sst with
+  | SymExState instk_height _ smem sstrg sctx sm => SymExState instk_height sstk smem sstrg sctx sm
+  end.
 
 Definition get_smemory_sst (sst: sstate) : smemory :=
-match sst with
-| SymExState _ _ smem _ _ _ => smem
-end.
+  match sst with
+  | SymExState _ _ smem _ _ _ => smem
+  end.
 
 Definition set_smemory_sst (sst: sstate) (smem: smemory) : sstate :=
-match sst with
-| SymExState instk_height sstk _ sstrg sctx sm => SymExState instk_height sstk smem sstrg sctx sm
-end.
+  match sst with
+  | SymExState instk_height sstk _ sstrg sctx sm => SymExState instk_height sstk smem sstrg sctx sm
+  end.
 
 Definition get_sstore_sst (sst : sstate) : sstorage :=
-match sst with
-| SymExState _ _ _ sstrg _ _ => sstrg
-end.
+  match sst with
+  | SymExState _ _ _ sstrg _ _ => sstrg
+  end.
 
 Definition set_sstore_sst (sst : sstate) (sstrg: sstorage) : sstate :=
-match sst with
-| SymExState instk_height sstk smem _ sctx sm => SymExState instk_height sstk smem sstrg sctx sm
-end.
+  match sst with
+  | SymExState instk_height sstk smem _ sctx sm => SymExState instk_height sstk smem sstrg sctx sm
+  end.
 
 Definition get_scontext_sst (sst : sstate) : scontext :=
-match sst with
-| SymExState _ _ _ _ sctx _ => sctx
-end.
+  match sst with
+  | SymExState _ _ _ _ sctx _ => sctx
+  end.
 
 Definition set_scontext_sst (sst : sstate) (sctx: scontext) : sstate :=
-match sst with
-| SymExState instk_height sstk smem sstrg _ sm => SymExState instk_height sstk smem sstrg sctx sm
-end.
+  match sst with
+  | SymExState instk_height sstk smem sstrg _ sm => SymExState instk_height sstk smem sstrg sctx sm
+  end.
 
 Definition get_smap_sst (sst : sstate) : smap :=
-match sst with
-| SymExState _ _ _ _ _ sm => sm
-end.
+  match sst with
+  | SymExState _ _ _ _ _ sm => sm
+  end.
 
 Definition set_smap_sst (sst : sstate) (sm: smap) : sstate :=
-match sst with
-| SymExState instk_height sstk smem sstrg sctx _ => SymExState instk_height sstk smem sstrg sctx sm
-end.
+  match sst with
+  | SymExState instk_height sstk smem sstrg sctx _ => SymExState instk_height sstk smem sstrg sctx sm
+  end.
 
 Definition add_to_smap (sm : smap) (value : smap_value) : prod nat smap :=
-  pair 0 (SymMap 0 []).
+  match sm with
+  | SymMap maxid map =>
+      let sm' := SymMap (S maxid) ((pair maxid value)::map) in
+       pair maxid sm'
+  end.
 
 
 (************)
@@ -976,28 +990,28 @@ Definition push_s (value : EVMWord) (sst : sstate) : option sstate :=
   end.
 
 Definition pop_s (sst : sstate): option sstate :=
-let sstk := get_sstack_sst sst in
-match pop sstk with
- | None => None
- | Some sstk' => Some (set_sstack_sst sst sstk')
-end.
+  let sstk := get_sstack_sst sst in
+  match pop sstk with
+  | None => None
+  | Some sstk' => Some (set_sstack_sst sst sstk')
+  end.
 
-Definition dup_s (k : nat) (sst : sstate) : option sstate  :=
-let sstk := get_sstack_sst sst in
-match dup k sstk with
- | None => None
- | Some sstk' => Some (set_sstack_sst sst sstk')
-end.
+Definition dup_s (k : nat) (sst : sstate) : option sstate :=
+  let sstk := get_sstack_sst sst in
+  match dup k sstk with
+  | None => None
+  | Some sstk' => Some (set_sstack_sst sst sstk')
+  end.
 
 Definition swap_s (k : nat) (sst : sstate) : option sstate :=
-let sstk := get_sstack_sst sst in
-match swap k sstk with
- | None => None
- | Some sstk' => Some (set_sstack_sst sst sstk')
-end.
+  let sstk := get_sstack_sst sst in
+  match swap k sstk with
+  | None => None
+  | Some sstk' => Some (set_sstack_sst sst sstk')
+  end.
 
 Definition mload_s (sst : sstate) : option sstate :=
-  let sm   : smap := get_smap_sst sst in
+  let sm : smap := get_smap_sst sst in
   let smem : smemory := get_smemory_sst sst in
   match get_sstack_sst sst with
   | offset::sstk =>
@@ -1012,7 +1026,7 @@ Definition mload_s (sst : sstate) : option sstate :=
   end.
 
 Definition sload_s (sst : sstate) : option sstate :=
-  let sm    : smap := get_smap_sst sst in
+  let sm : smap := get_smap_sst sst in
   let sstrg : sstorage := get_sstore_sst sst in
   match get_sstack_sst sst with
   | skey::sstk =>
@@ -1027,7 +1041,7 @@ Definition sload_s (sst : sstate) : option sstate :=
   end.
 
 Definition sha3_s (sst : sstate) : option sstate :=
-  let sm   : smap := get_smap_sst sst in
+  let sm : smap := get_smap_sst sst in
   let smem : smemory := get_smemory_sst sst in
   match get_sstack_sst sst with
   | offset::size::sstk =>
@@ -1038,12 +1052,11 @@ Definition sha3_s (sst : sstate) : option sstate :=
           let sst'' := set_smap_sst sst sm' in
           Some sst'
       end
-  | _ => None
-  end.
+  | _ => None end.
 
 Definition mstore8_s (sst : sstate) : option sstate :=
   match get_sstack_sst sst with
-  | offset::value::sstk => 
+  | offset::value::sstk =>
       let smem := get_smemory_sst sst in
       let st' := set_smemory_sst sst ((SymMSTORE8 offset value)::smem) in
       let st'' := set_sstack_sst sst sstk in
@@ -1053,7 +1066,7 @@ Definition mstore8_s (sst : sstate) : option sstate :=
       
 Definition mstore_s (sst : sstate) : option sstate :=
   match get_sstack_sst sst with
-  | offset::value::sstk => 
+  | offset::value::sstk =>
       let smem := get_smemory_sst sst in
       let st' := set_smemory_sst sst ((SymMSTORE offset value)::smem) in
       let st'' := set_sstack_sst sst sstk in
@@ -1061,9 +1074,9 @@ Definition mstore_s (sst : sstate) : option sstate :=
   | _ => None
   end.
 
-Definition sstore_s (sst : sstate) : option sstate := 
+Definition sstore_s (sst : sstate) : option sstate :=
   match get_sstack_sst sst with
-  | key::value::sstk => 
+  | key::value::sstk =>
       let sstrg := get_sstore_sst sst in
       let st' := set_sstore_sst sst ((SymSSTORE key value)::sstrg) in
       let st'' := set_sstack_sst sst sstk in
@@ -1071,16 +1084,15 @@ Definition sstore_s (sst : sstate) : option sstate :=
   | _ => None
   end.
 
-
-Definition exec_op_s (sst : sstate) (ops : stack_op_map) (label : stack_op_instr) : option sstate :=
+Definition exec_op_s (sst : sstate) (ops : stack_op_instr_map) (label : stack_op_instr) : option sstate :=
   match (ops label) with
   | None => None
-  | Some (OpImp nb_args func _) => 
+  | Some (OpImp nb_args func _) =>
       let sstk := get_sstack_sst sst in
-      match firstn_e nb_args sstk, skipn_e nb_args sstk with          
-      | Some s1, Some s2 =>
-          let sm : smap := get_smap_sst sst in              
-          let v  : smap_value := SymOp label s1 in
+      match firstn_e nb_args sstk, skipn_e nb_args sstk with
+      | Some s1,Some s2 =>
+          let sm : smap := get_smap_sst sst in
+          let v : smap_value := SymOp label s1 in
           match add_to_smap sm v with
           | pair key sm' =>
               let sst' := set_sstack_sst sst ((FreshVar key)::s2) in
@@ -1091,18 +1103,32 @@ Definition exec_op_s (sst : sstate) (ops : stack_op_map) (label : stack_op_instr
       end
   end.
 
-Definition evm_sexec_inst (inst: instr) (sst: sstate) (ops: stack_op_map) : option sstate :=
+Definition evm_sexec_instr (inst: instr) (sst: sstate) (ops: stack_op_instr_map) : option sstate :=
   match inst with
   | PUSH size w => push_s (NToWord EVMWordSize w) sst
   | POP => pop_s sst
   | DUP pos => dup_s pos sst
   | SWAP pos => swap_s pos sst
-  | MLOAD => mload_s sst                 
-  | MSTORE8 => mstore8_s sst                 
-  | MSTORE => mstore_s sst                 
-  | SLOAD => sload_s sst                 
+  | MLOAD => mload_s sst
+  | MSTORE8 => mstore8_s sst
+  | MSTORE => mstore_s sst
+  | SLOAD => sload_s sst
   | SSTORE => sstore_s sst
   | SHA3 => sha3_s sst
   | KECCAK256 => sha3_s sst
   | OpInstr label => exec_op_s sst ops label
   end.
+
+Fixpoint evm_sexec_block' (p : block) (sst : sstate) (ops : stack_op_instr_map) : option sstate :=
+  match p with
+  | [] => Some sst
+  | inste::instrs' =>
+      match (evm_sexec_instr inste sst ops) with
+      | None => None
+      | Some sst' => evm_sexec_block' instrs' sst' ops
+      end
+  end.
+
+Definition evm_sexec_block (p : block) (instk_height: nat) (ops : stack_op_instr_map) : option sstate :=
+  let sst := gen_empty_sstate instk_height in 
+  evm_sexec_block' p sst ops.
